update Hoare2.v

programming_language_foundations/Hoare2.v
@@ -9,4 +9,98 @@ From Coq Require Import Arith.EqNat.
 From Coq Require Import Arith.PeanoNat. Import Nat.
 From Coq Require Import omega.Omega.
 From PLF Require Import Hoare.
-From PLF Require Import Imp.
+From LF Require Import Imp.
+
+Definition reduce_to_zero' : com :=
+  (WHILE ~( X = 0) DO
+     X ::= X - 1
+   END)%imp.
+
+Theorem reduce_to_zero_correct' :
+  {{fun st => True}}
+    reduce_to_zero'
+  {{fun st => st X = 0}}.
+Proof.
+  unfold reduce_to_zero'.
+  eapply hoare_consequence_post.
+  - apply hoare_while.
+    eapply hoare_consequence_pre.
+    + apply hoare_asgn.
+    + unfold assert_implies, assn_sub. auto.
+  - unfold assert_implies.
+    intros st [_ H].
+    unfold bassn in H. simpl in H.
+    apply eq_true_negb_classical in H.
+    rewrite eqb_eq in H. apply H.
+Qed.
+
+Fixpoint parity x :=
+  match x with
+  | 0 => 0
+  | 1 => 1
+  | S (S x') => parity x'
+  end.
+
+Lemma parity_ge_2 : forall x,
+    2 <= x -> parity (x - 2) = parity x.
+Proof.
+  intros x H.
+  induction x as [|x' IH].
+  - omega.
+  - destruct x' as [|x''].
+    + omega.
+    + simpl. rewrite sub_0_r. reflexivity.
+Qed.
+
+Lemma parity_lt_2 : forall x,
+    ~ 2 <= x ->
+    parity (x) = x.
+Proof.
+  intros x H.
+  destruct x as [| x'].
+  - reflexivity.
+  - destruct x' as [|x''].
+    + reflexivity.
+    + omega.
+Qed.
+
+Theorem parity_correct : forall m,
+    {{fun st => st X = m}}
+      WHILE 2 <= X DO
+        X ::= X - 2
+      END
+    {{fun st => st X = parity m}}.
+Proof.
+  intro m.
+  eapply hoare_consequence_post.
+  - eapply hoare_consequence_pre.
+    + Print hoare_while.
+      apply (hoare_while (fun st => parity (st X) = parity m)).
+      eapply hoare_consequence_pre.
+      * apply hoare_asgn.
+      * unfold assert_implies, assn_sub.
+        intros st [H1 H2].
+        rewrite t_update_eq.
+        simpl in *. rewrite <- H1.
+        apply parity_ge_2.
+        unfold bassn in H2.
+        simpl in H2.
+        destruct (st X).
+        { inversion H2. }
+        { destruct n.
+          { inversion H2. }
+          { omega. }
+        }
+    + unfold assert_implies.
+      intros st H.
+      rewrite H. reflexivity.
+  - unfold assert_implies.
+    intros st [H1 H2].
+    unfold bassn in H2.
+    simpl in H2. destruct (st X).
+    + simpl in H1. apply H1.
+    + destruct n.
+      * simpl in H1. apply H1.
+      * exfalso. apply H2. reflexivity.
+Qed.
+
